Remove notations like =? in AsciiOrder and StringOrder
 These notations already exist in Coq 8.9, causing a nasty warning

StringOrder.v
@@ -8,11 +8,14 @@ Require Import Bool Orders Ascii AsciiOrder String.
 Local Open Scope string_scope.
 
 Inductive string_lt : string -> string -> Prop :=
- | LtEmpty a s : "" < String a s
- | LtHead a a' s s' : (a < a')%char -> String a s < String a' s'
- | LtTail a s s' : s < s' -> String a s < String a s'
-where "u < v" := (string_lt u v) : string_scope.
+ | LtEmpty a s : string_lt "" (String a s)
+ | LtHead a a' s s' : ascii_lt a a' -> string_lt (String a s) (String a' s')
+ | LtTail a s s' : string_lt s s' -> string_lt (String a s) (String a s').
 Hint Constructors string_lt.
+Local Infix "<" := string_lt.
+
+Definition string_le s s' := s<s' \/ s=s'.
+Local Infix "<=" := string_le.
 
 Lemma string_lt_strorder : StrictOrder string_lt.
 Proof.
@@ -22,9 +25,6 @@ Proof.
  - red. intros x y z H; revert z. induction H; inversion_clear 1; auto.
    constructor. eapply ascii_lt_strorder; eauto.
 Qed.
-
-Definition string_le s s' := s<s' \/ s=s'.
-Infix "<=" := string_le : string_scope.
 
 Lemma string_le_lteq s s' : s<=s' <-> s<s' \/ s=s'.
 Proof.
@@ -37,17 +37,15 @@ Fixpoint string_compare s s' :=
   | "", _ => Lt
   | _, "" => Gt
   | String a s, String a' s' =>
-    match (a ?= a')%char with
+    match ascii_compare a a' with
     | Eq => string_compare s s'
     | Lt => Lt
     | Gt => Gt
     end
   end.
 
-Infix "?=" := string_compare (at level 70) : string_scope.
-
 Lemma string_compare_spec s s' :
- CompareSpec (s=s') (s<s') (s'<s) (s?=s').
+ CompareSpec (s=s') (s<s') (s'<s) (string_compare s s').
 Proof.
  revert s'.
  induction s as [|a s IH]; destruct s' as [|a' s']; simpl; auto.
@@ -56,28 +54,24 @@ Proof.
 Qed.
 
 Definition string_eqb s s' :=
- match s ?= s' with
+ match string_compare s s' with
  | Eq => true
  | _ => false
  end.
 
 Definition string_ltb s s' :=
- match s ?= s' with
+ match string_compare s s' with
  | Lt => true
  | _ => false
  end.
 
 Definition string_leb s s' :=
- match s ?= s' with
+ match string_compare s s' with
  | Gt => false
  | _ => true
  end.
 
-Infix "=?" := string_eqb : string_scope.
-Infix "<?" := string_ltb : string_scope.
-Infix "<=?" := string_leb : string_scope.
-
-Lemma string_eqb_spec (s s' : string) : reflect (s = s') (s =? s').
+Lemma string_eqb_spec s s' : reflect (s = s') (string_eqb s s').
 Proof.
  unfold string_eqb.
  assert (H := string_compare_spec s s').
@@ -86,14 +80,14 @@ Proof.
  intros <-. assert (~(s < s)) by apply string_lt_strorder. auto.
 Qed.
 
-Lemma string_ltb_spec (s s' : string) : BoolSpec (s < s') (s' <= s) (s <? s').
+Lemma string_ltb_spec s s' : BoolSpec (s < s') (s' <= s) (string_ltb s s').
 Proof.
  unfold string_ltb, string_le.
  assert (H := string_compare_spec s s').
  destruct string_compare; constructor; inversion H; auto.
 Qed.
 
-Lemma string_leb_spec (s s' : string) : BoolSpec (s <= s') (s' < s) (s <=? s').
+Lemma string_leb_spec s s' : BoolSpec (s <= s') (s' < s) (string_leb s s').
 Proof.
  unfold string_leb, string_le.
  assert (H := string_compare_spec s s').
